src/dafny/util/int.dfy
@@ -94,11 +94,111 @@ module Int {
     var b2 := read_u32(bytes, address+4) as u64;
     (b1 * (TWO_32 as u64)) + b2
   }
+
+
+  // =========================================================
+  // Non-Euclidean Division / Remainder
+  // =========================================================
+
+  // This provides a non-Euclidean division operator and is necessary
+  // because Dafny (unlike just about every other programming
+  // language) supports Euclidean division.  This operator, therefore,
+  // always divides *towards* zero.
+  function method div(lhs: int, rhs: int) : int
+  requires rhs != 0 {
+    if lhs >= 0 then lhs / rhs
+    else
+      -((-lhs) / rhs)
+  }
+
+  // This provides a non-Euclidean remainder operator and is necessary
+  // because Dafny (unlike just about every other programming
+  // language) supports Euclidean division.  Observe that this is a
+  // true remainder operator, and not a modulus operator.  For
+  // emxaple, this means the result can be negative.
+  function method rem(lhs: int, rhs: int) : int
+  requires rhs != 0 {
+    if lhs >= 0 then (lhs % rhs)
+    else
+      var d := -((-lhs) / rhs);
+      lhs - (d * rhs)
+  }
+
+  // Various sanity tests for division.
+  method div_tests() {
+    // pos-pos
+    assert div(6,2) == 3;
+    assert div(6,3) == 2;
+    assert div(6,4) == 1;
+    assert div(9,4) == 2;
+    // neg-pos
+    assert div(-6,2) == -3;
+    assert div(-6,3) == -2;
+    assert div(-6,4) == -1;
+    assert div(-9,4) == -2;
+    // pos-neg
+    assert div(6,-2) == -3;
+    assert div(6,-3) == -2;
+    assert div(6,-4) == -1;
+    assert div(9,-4) == -2;
+    // neg-neg
+    assert div(-6,-2) == 3;
+    assert div(-6,-3) == 2;
+    assert div(-6,-4) == 1;
+    assert div(-9,-4) == 2;
+  }
+
+  // Various sanity tests for remainder.
+  method rem_tests() {
+    // pos-pos
+    assert rem(6,2) == 0;
+    assert rem(6,3) == 0;
+    assert rem(6,4) == 2;
+    assert rem(9,4) == 1;
+    // neg-pos
+    assert rem(-6,2) == 0;
+    assert rem(-6,3) == 0;
+    assert rem(-6,4) == -2;
+    assert rem(-9,4) == -1;
+    // pos-neg
+    assert rem(6,-2) == 0;
+    assert rem(6,-3) == 0;
+    assert rem(6,-4) == 2;
+    assert rem(9,-4) == 1;
+    // neg-neg
+    assert rem(-6,-2) == 0;
+    assert rem(-6,-3) == 0;
+    assert rem(-6,-4) == -2;
+    assert rem(-9,-4) == -1;
+  }
 }
 
-// =========================================================
-// Conversion from words (i.e. raw data) to signed data
-// =========================================================
+module I256 {
+  import opened Int
+
+  // This provides a non-Euclidean division operator and is necessary
+  // because Dafny (unlike just about every other programming
+  // language) supports Euclidean division.  This operator, therefore,
+  // always divides *towards* zero.
+  function method div(lhs: i256, rhs: i256) : i256
+    // Cannot divide by zero!
+    requires rhs != 0
+    // Range restriction to prevent overflow
+    requires (rhs != -1 || lhs != (-TWO_255 as i256)) {
+    Int.div(lhs as int, rhs as int) as i256
+  }
+
+  // This provides a non-Euclidean remainder operator and is necessary
+  // because Dafny (unlike just about every other programming
+  // language) supports Euclidean division.  Observe that this is a
+  // true remainder operator, and not a modulus operator.  For
+  // emxaple, this means the result can be negative.
+  function method rem(lhs: i256, rhs: i256) : i256
+    // Cannot divide by zero!
+    requires rhs != 0 {
+    Int.rem(lhs as int, rhs as int) as i256
+  }
+}
 
 module Word {
   import opened Int
